thys/Context_Free_Grammar/Expansion.thy
@@ -6,32 +6,39 @@ begin
 
 section \<open>Expansion of Grammars\<close>
 
+lemma conc_eq_empty_iff: "X @@ Y = {} \<longleftrightarrow> X = {} \<or> Y = {}"
+  by auto
+
+lemma Nts_syms_conc: "\<Union>(Nts_syms ` (X @@ Y)) =
+ (if X = {} \<or> Y = {} then {} else \<Union>(Nts_syms ` X) \<union> \<Union>(Nts_syms ` Y))"
+  by (force elim!: concE)
+
 text \<open>We consider the set of admissible expansions of grammars.
 
 For a symbol,
 one option is not to expand it,
-and the other option for (unlocked) nonterminals is to expand to the all rhss.\<close>
+and the other option for (expandable) nonterminals is to expand to the all rhss.\<close>
 
 definition Expand_sym_ops :: "('n,'t) Prods \<Rightarrow> 'n set \<Rightarrow> ('n,'t) sym \<Rightarrow> ('n,'t) syms set set" where
-"Expand_sym_ops P L x =
-  insert {[x]} (case x of Nt A \<Rightarrow> if A \<in> L then {} else {Rhss P A} | _ \<Rightarrow> {})"
+"Expand_sym_ops P X x =
+  insert {[x]} (case x of Nt A \<Rightarrow> if A \<in> X then {Rhss P A} else {} | _ \<Rightarrow> {})"
 
 lemma Expand_sym_ops_simps:
-  "Expand_sym_ops P L (Tm a) = {{[Tm a]}}"
-  "Expand_sym_ops P L (Nt A) = insert {[Nt A]} (if A \<in> L then {} else {Rhss P A})"
+  "Expand_sym_ops P X (Tm a) = {{[Tm a]}}"
+  "Expand_sym_ops P X (Nt A) = insert {[Nt A]} (if A \<in> X then {Rhss P A} else {})"
   by (auto simp: Expand_sym_ops_def)
 
-lemma Expand_sym_ops_self: "{[x]} \<in> Expand_sym_ops P L x"
+lemma Expand_sym_ops_self: "{[x]} \<in> Expand_sym_ops P X x"
   by (simp add: Expand_sym_ops_def)
 
 text \<open>Mixed words allow all possible combinations of the options for the symbols.\<close>
 
 fun Expand_syms_ops :: "('n,'t) Prods \<Rightarrow> 'n set \<Rightarrow> ('n,'t) syms \<Rightarrow> ('n,'t) syms set set" where
-  "Expand_syms_ops P L [] = {{[]}}"
-| "Expand_syms_ops P L (x#xs) =
-   {\<alpha>s @@ \<beta>s | \<alpha>s \<beta>s. \<alpha>s \<in> Expand_sym_ops P L x \<and> \<beta>s \<in> Expand_syms_ops P L xs}"
+  "Expand_syms_ops P X [] = {{[]}}"
+| "Expand_syms_ops P X (x#xs) =
+   {\<alpha>s @@ \<beta>s | \<alpha>s \<beta>s. \<alpha>s \<in> Expand_sym_ops P X x \<and> \<beta>s \<in> Expand_syms_ops P X xs}"
 
-lemma Expand_syms_ops_self: "{\<alpha>} \<in> Expand_syms_ops P L \<alpha>"
+lemma Expand_syms_ops_self: "{\<alpha>} \<in> Expand_syms_ops P X \<alpha>"
 proof (induction \<alpha>)
   case Nil
   show ?case by simp
@@ -42,11 +49,11 @@ next
 qed
 
 lemma Expand_sym_ops_Lang_of_Cons:
-  assumes X: "X \<in> Expand_sym_ops P L x" and L: "Lhss Q \<subseteq> L"
-  shows "Lang_of (P \<union> Q) (x#xs) = Lang_of_set (P \<union> Q) X @@ Lang_of (P \<union> Q) xs"
+  assumes U: "U \<in> Expand_sym_ops P X x" and X: "Lhss Q \<inter> X = {}"
+  shows "Lang_of (P \<union> Q) (x#xs) = Lang_of_set (P \<union> Q) U @@ Lang_of (P \<union> Q) xs"
 proof-
-  { fix A assume "A \<notin> L"
-    with L have "A \<notin> Lhss Q" by auto
+  { fix A assume "A \<in> X"
+    with X have "A \<notin> Lhss Q" by auto
     then have "Rhss (P \<union> Q) A = Rhss P A" by (auto simp: Rhss_Un notin_Lhss_iff_Rhss)
     with Lang_of_set_Rhss[of "P \<union> Q" A]
     have "Lang_of_set (P \<union> Q) (Rhss P A) = Lang (P \<union> Q) A" by auto
@@ -57,41 +64,49 @@ proof-
 qed
 
 lemma Expand_syms_ops_Lang_of:
-  assumes X: "X \<in> Expand_syms_ops P L \<alpha>" and L: "Lhss Q \<subseteq> L"
-  shows "Lang_of (P \<union> Q) \<alpha> = Lang_of_set (P \<union> Q) X"
-proof (insert X, induction \<alpha> arbitrary: X)
+  assumes U: "U \<in> Expand_syms_ops P L \<alpha>" and L: "Lhss Q \<inter> L = {}"
+  shows "Lang_of (P \<union> Q) \<alpha> = Lang_of_set (P \<union> Q) U"
+proof (insert U, induction \<alpha> arbitrary: U)
   case Nil
   then show ?case by simp
 next
   case (Cons x \<alpha>)
-  from Cons.prems obtain Y Z
-    where X: "X = Y @@ Z"
-      and Y: "Y \<in> Expand_sym_ops P L x"
-      and Z: "Z \<in> Expand_syms_ops P L \<alpha>"
+  from Cons.prems obtain V W
+    where U: "U = V @@ W"
+      and V: "V \<in> Expand_sym_ops P L x"
+      and W: "W \<in> Expand_syms_ops P L \<alpha>"
     by auto
-  show ?case by (simp add: X Cons.IH[OF Z] Expand_sym_ops_Lang_of_Cons[OF Y L] Lang_of_set_conc)
+  show ?case by (simp add: U Cons.IH[OF W] Expand_sym_ops_Lang_of_Cons[OF V L] Lang_of_set_conc)
 qed
 
 definition Expand :: "(('n,'t) syms \<Rightarrow> ('n,'t) syms set) \<Rightarrow> ('n,'t) Prods \<Rightarrow> ('n,'t) Prods" where
-"Expand f Q = (\<Union>(A,\<alpha>) \<in> Q. Pair A ` f \<alpha>)"
+"Expand f P = {(A,\<alpha>') |A \<alpha>'. \<exists>\<alpha>. (A,\<alpha>) \<in> P \<and> \<alpha>' \<in> f \<alpha>}"
 
-lemma Lhss_Expand: "Lhss (Expand f Q) \<subseteq> Lhss Q"
+lemma Expand_eq_UN[code]:
+  "Expand f P = (\<Union>(A,\<alpha>) \<in> P. Pair A ` f \<alpha>)"
+  by (auto simp: Expand_def)
+
+lemma Expand_via_Rhss:
+  "Expand f P = {(A,\<alpha>). \<alpha> \<in> \<Union>(f ` Rhss P A)}"
+  by (auto simp: Expand_def Rhss_def)
+
+lemma Lhss_Expand: "Lhss (Expand f P) \<subseteq> Lhss P"
   by (auto simp: Lhss_def Expand_def split: prod.splits)
 
-lemma Rhss_Expand: "Rhss (Expand f Q) A = \<Union>(f ` Rhss Q A)"
+lemma Rhss_Expand: "Rhss (Expand f P) A = \<Union>(f ` Rhss P A)"
   by (auto simp: Rhss_def Expand_def)
 
-lemma Rhs_Nts_Expand: "Rhs_Nts (Expand f Q) = (\<Union>(A,\<alpha>) \<in> Q. \<Union>\<beta> \<in> f \<alpha>. Nts_syms \<beta>)"
+lemma Rhs_Nts_Expand: "Rhs_Nts (Expand f P) = (\<Union>(A,\<alpha>) \<in> P. \<Union>\<beta> \<in> f \<alpha>. Nts_syms \<beta>)"
   by (auto simp: Expand_def Rhs_Nts_def)
 
 text \<open>When each production is expanded in an admissible way,
 then the language is preserved.\<close>
 
 definition Expand_ops :: "('n,'t) Prods \<Rightarrow> 'n set \<Rightarrow> (('n,'t) syms \<Rightarrow> ('n,'t) syms set) set" where
-"Expand_ops P L = {f. \<forall>\<alpha>. f \<alpha> \<in> Expand_syms_ops P L \<alpha>}"
+"Expand_ops P X = {f. \<forall>\<alpha>. f \<alpha> \<in> Expand_syms_ops P X \<alpha>}"
 
 theorem Lang_Un_Expand:
-  assumes f: "f \<in> Expand_ops P L" and L: "Lhss Q \<subseteq> L"
+  assumes f: "f \<in> Expand_ops P X" and X: "X \<inter> Lhss Q = {}"
   shows "Lang (P \<union> Expand f Q) = Lang (P \<union> Q)"
   unfolding Lang_eq_iff_Lang_of_eq
 proof (safe intro!: ext elim!: Lang_ofE_deriven)
@@ -136,7 +151,7 @@ proof (safe intro!: ext elim!: Lang_ofE_deriven)
           by (auto simp: Lang_of_def)
         also have "\<dots> = Lang_of (P \<union> Q) \<alpha>"
           apply (subst Expand_syms_ops_Lang_of)
-          using f AQ L by (auto simp: Expand_ops_def)
+          using f AQ X by (auto simp: Expand_ops_def)
         also have "\<dots> \<subseteq> Lang (P \<union> Q) A"
           apply (rule Lang_of_prod_subset)
           using AQ by auto
@@ -182,10 +197,10 @@ next
       next
         case False
         with A\<alpha> have A\<alpha>Q: "(A,\<alpha>) \<in> Q" by simp
-        with f have f\<alpha>: "f \<alpha> \<in> Expand_syms_ops P L \<alpha>" by (auto simp: Expand_ops_def)
-        from L Lhss_Expand[of f Q]
-        have Lhss: "Lhss (Expand f Q) \<subseteq> L" by auto
-        from L A\<alpha>Q have Rhss: "f \<alpha> \<subseteq> Rhss (Expand f Q) A"
+        with f have f\<alpha>: "f \<alpha> \<in> Expand_syms_ops P X \<alpha>" by (auto simp: Expand_ops_def)
+        from X Lhss_Expand[of f Q]
+        have Lhss: "Lhss (Expand f Q) \<inter> X = {}" by auto
+        from X A\<alpha>Q have Rhss: "f \<alpha> \<subseteq> Rhss (Expand f Q) A"
           by (auto simp: Rhss_def Expand_def)
         from u Expand_syms_ops_Lang_of[OF f\<alpha> Lhss]
         have "u \<in> Lang_of_set (P \<union> Expand f Q) (f \<alpha>)" by auto
@@ -199,16 +214,16 @@ next
 qed
 
 corollary Lang_Expand_Un:
-  assumes f: "f \<in> Expand_ops P L" and L: "Lhss Q \<subseteq> L"
+  assumes "f \<in> Expand_ops P X" and "X \<inter> Lhss Q = {}"
   shows "Lang (Expand f Q \<union> P) = Lang (Q \<union> P)"
-  using Lang_Un_Expand[OF f L] by (simp add: ac_simps)
+  using Lang_Un_Expand[OF assms] by (simp add: ac_simps)
 
 subsection \<open>Instances\<close>
 
 text \<open>For symbols, we just provide a function to expand it.\<close>
 
 definition Expand_sym :: "('n,'t) Prods \<Rightarrow> 'n set \<Rightarrow> ('n,'t) sym \<Rightarrow> ('n,'t) syms set" where
-"Expand_sym P L x = (case x of Nt A \<Rightarrow> if A \<in> L then {[x]} else Rhss P A | _ \<Rightarrow> {[x]})"
+"Expand_sym P X x = (case x of Nt A \<Rightarrow> if A \<in> X then Rhss P A else {[x]} | _ \<Rightarrow> {[x]})"
 
 lemma Expand_sym_ops: "Expand_sym P L x \<in> Expand_sym_ops P L x"
   by (auto simp: Expand_sym_def Expand_sym_ops_simps split: sym.splits)
@@ -216,37 +231,160 @@ lemma Expand_sym_ops: "Expand_sym P L x \<in> Expand_sym_ops P L x"
 subsubsection \<open>Expanding all nonterminals\<close>
 
 fun Expand_all_syms :: "('n,'t) Prods \<Rightarrow> 'n set \<Rightarrow> ('n,'t) syms \<Rightarrow> ('n,'t) syms set" where
-  "Expand_all_syms P L [] = {[]}"
-| "Expand_all_syms P L (x#xs) = Expand_sym P L x @@ Expand_all_syms P L xs"
+  "Expand_all_syms P X [] = {[]}"
+| "Expand_all_syms P X (x#xs) = Expand_sym P X x @@ Expand_all_syms P X xs"
 
-lemma Expand_all_syms_ops: "Expand_all_syms P L xs \<in> Expand_syms_ops P L xs"
-  by (induction xs, simp, force simp: Expand_sym_ops)
+lemma Expand_all_syms_eq_foldr:
+  "Expand_all_syms P X \<alpha> = foldr (@@) (map (Expand_sym P X) \<alpha>) {[]}"
+  by (induction \<alpha>, simp_all)
 
-lemma Expand_all_ops: "Expand_all_syms P L \<in> Expand_ops P L"
+lemma Expand_all_syms_append:
+  "Expand_all_syms P X (\<alpha>@\<beta>) = Expand_all_syms P X \<alpha> @@ Expand_all_syms P X \<beta>"
+  by (induction \<alpha> arbitrary: \<beta>, simp_all add: conc_assoc)
+
+lemma Expand_all_syms_ops: "Expand_all_syms P X \<alpha> \<in> Expand_syms_ops P X \<alpha>"
+  by (induction \<alpha>, simp, force simp: Expand_sym_ops)
+
+lemma Expand_all_ops: "Expand_all_syms P X \<in> Expand_ops P X"
   by (auto simp: Expand_ops_def Expand_all_syms_ops)
 
 abbreviation Expand_all :: "('n,'t) Prods \<Rightarrow> 'n set \<Rightarrow> ('n,'t) Prods \<Rightarrow> ('n,'t) Prods" where
-  "Expand_all P L Q \<equiv> Expand (Expand_all_syms P L) Q"
+  "Expand_all P X Q \<equiv> Expand (Expand_all_syms P X) Q"
 
-theorem Lang_Expand_all:
-  assumes "Lhss Q \<subseteq> L"
-  shows "Lang (Expand_all P L Q \<union> P) = Lang (Q \<union> P)"
+corollary Lang_Un_Expand_all:
+  assumes "X \<inter> Lhss Q = {}"
+  shows "Lang (P \<union> Expand_all P X Q) = Lang (P \<union> Q)"
+  using Lang_Un_Expand[OF Expand_all_ops assms].
+
+corollary Lang_Expand_all_Un:
+  assumes "X \<inter> Lhss Q = {}"
+  shows "Lang (Expand_all P X Q \<union> P) = Lang (Q \<union> P)"
   using Lang_Expand_Un[OF Expand_all_ops assms].
+
+text \<open>@{term Expand_all} removes expanded nonterminals and adds those which the
+expanded nonterminals depends.\<close>
+
+lemma Expand_all_syms_eq_empty: "Expand_all_syms P X \<alpha> = {} \<longleftrightarrow> \<not> Nts_syms \<alpha> \<inter> X \<subseteq> Lhss P"
+  by (induction \<alpha>)
+    (auto simp: Expand_sym_def conc_eq_empty_iff notin_Lhss_iff_Rhss[symmetric] split: sym.splits)
+
+lemma Nts_syms_Expand_all:
+  "\<Union>(Nts_syms ` Expand_all_syms P X \<alpha>) =
+   (if Nts_syms \<alpha> \<inter> X \<subseteq> Lhss P
+    then Nts_syms \<alpha> - X \<union> \<Union>(Nts_syms ` \<Union>(Rhss P ` (Nts_syms \<alpha> \<inter> X)))
+    else {})"
+proof (induction \<alpha>)
+  case Nil
+  show ?case by simp
+next
+  case (Cons x \<alpha>)
+  then show ?case
+    by (auto simp: Expand_sym_def Nts_syms_conc Cons Expand_all_syms_eq_empty
+        notin_Lhss_iff_Rhss[symmetric] split: sym.splits)
+qed
+
+lemma Rhs_Nts_Expand_all:
+  "Rhs_Nts (Expand_all P X Q) =
+   (\<Union>(A,\<alpha>) \<in> Q. if Nts_syms \<alpha> \<inter> X \<subseteq> Lhss P
+    then Nts_syms \<alpha> - X \<union> \<Union>(Nts_syms ` \<Union>(Rhss P ` (Nts_syms \<alpha> \<inter> X)))
+    else {})"
+  apply (unfold Rhs_Nts_Expand)
+  apply (rule SUP_cong[OF refl])
+  apply (rule prod.case_cong[OF refl])
+  by (rule Nts_syms_Expand_all)
+
+lemma Rhs_Nts_Expand_all_le:
+  "Rhs_Nts (Expand_all P X Q) \<subseteq> Rhs_Nts Q - X \<union> \<Union>(Nts_syms ` \<Union>(Rhss P ` (Rhs_Nts Q \<inter> X)))"
+  (is "?l \<subseteq> ?r")
+proof-
+  have "?l \<subseteq> (\<Union>(A,\<alpha>) \<in> Q. Nts_syms \<alpha> - X \<union> \<Union>(Nts_syms ` \<Union>(Rhss P ` (Nts_syms \<alpha> \<inter> X))))"
+    apply (unfold Rhs_Nts_Expand_all)
+    apply (rule SUP_mono')
+    by (auto simp: if_splits)
+  also have "\<dots> = ?r" by (auto simp: Rhs_Nts_def)
+  finally show ?thesis.
+qed
+
+text \<open>Approximately, \<open>Expand_all\<close> depends on nonterminals that are not expanded and
+those that the expanding grammar depends.\<close>
+
+lemma Rhs_Nts_Expand_all_le_Rhs_Nts:
+  "Rhs_Nts (Expand_all P X Q) \<subseteq> Rhs_Nts Q - X \<union> Rhs_Nts P"
+  (is "?l \<subseteq> ?r")
+proof-
+  note Rhs_Nts_Expand_all_le
+  also have "Rhs_Nts Q - X \<union> \<Union>(Nts_syms ` \<Union>(Rhss P ` (Rhs_Nts Q \<inter> X))) \<subseteq> ?r"
+    by (auto simp: Rhss_def Rhs_Nts_def)
+  finally show ?thesis.
+qed
+
+text \<open>One can remove a non-recursive part of grammar by expanding others
+with respect to it.\<close>
+
+lemma Lang_Expand_all_idem:
+  assumes PP: "Rhs_Nts P \<inter> Lhss P = {}"
+    and PQ: "Lhss P \<inter> Lhss Q = {}" and AP: "A \<notin> Lhss P"
+  shows "Lang (Expand_all P (Lhss P) Q) A = Lang (P \<union> Q) A"
+  (is "?l = ?r")
+proof-
+  have "?l = Lang (P \<union> Expand_all P (Lhss P) Q) A"
+    apply (rule Lang_disj_Lhss_Un[symmetric])
+    using Rhs_Nts_Expand_all_le_Rhs_Nts[of P "Lhss P" Q] PP AP by auto
+  also have "\<dots> = Lang (P \<union> Q) A" by (simp add: Lang_Un_Expand_all[OF PQ])
+  finally show ?thesis.
+qed
+
+lemma Lang_of_Expand_all_idem:
+  assumes PP: "Rhs_Nts P \<inter> Lhss P = {}" and PQ: "Lhss P \<inter> Lhss Q = {}"
+    and AP: "Nts_syms \<alpha> \<inter> Lhss P = {}"
+  shows "Lang_of (Expand_all P (Lhss P) Q) \<alpha> = Lang_of (P \<union> Q) \<alpha>"
+  apply (insert AP, induction \<alpha>)
+  using Lang_Expand_all_idem[OF PP PQ]
+  by (simp_all split: sym.splits add: Lang_of_Cons)
+
+lemma Lang_Expand_all_idem_new:
+  assumes PP: "Rhs_Nts P \<inter> Lhss P = {}" and PQ: "Lhss P \<inter> Lhss Q = {}"
+    and AP: "A \<in> Lhss P"
+  shows "Lang_of_set (Expand_all P (Lhss P) Q) (Rhss P A) = Lang (P \<union> Q) A"
+    (is "?l = ?r")
+proof-
+  have "\<alpha> \<in> Rhss P A \<Longrightarrow> Lang_of (Expand_all P (Lhss P) Q) \<alpha> = Lang_of (P \<union> Q) \<alpha>" for \<alpha>
+    apply (rule Lang_of_Expand_all_idem[OF PP PQ])
+    using PP by (auto simp: Rhss_def Rhs_Nts_def)
+  then have "?l = Lang_of_set (P \<union> Q) (Rhss P A)" by auto
+  moreover have "Rhss P A = Rhss (P \<union> Q) A" using AP PQ by (auto simp: Rhss_def dest: in_LhssI)
+  ultimately show ?thesis by (simp add: Lang_of_set_Rhss)
+qed
+
+lemma Lang_idem_Un_via_Expand_all:
+  assumes PP: "Rhs_Nts P \<inter> Lhss P = {}" and PQ: "Lhss P \<inter> Lhss Q = {}"
+  shows "Lang (P \<union> Q) A =
+    (if A \<in> Lhss P then Lang_of_set (Expand_all P (Lhss P) Q) (Rhss P A)
+     else Lang (Expand_all P (Lhss P) Q) A)"
+  using Lang_Expand_all_idem[OF assms] Lang_Expand_all_idem_new[OF assms]
+  by auto
+
+corollary Lang_Un_idem_via_Expand_all:
+  assumes PQ: "Lhss P \<inter> Lhss Q = {}" and QQ: "Rhs_Nts Q \<inter> Lhss Q = {}"
+  shows "Lang (P \<union> Q) A =
+    (if A \<in> Lhss Q then Lang_of_set (Expand_all Q (Lhss Q) P) (Rhss Q A)
+     else Lang (Expand_all Q (Lhss Q) P) A)"
+  using Lang_idem_Un_via_Expand_all[of Q P A] assms by (auto simp: ac_simps)
 
 subsubsection \<open>Expanding head nonterminals\<close>
 
 definition Expand_hd_syms :: "('n,'t) Prods \<Rightarrow> 'n set \<Rightarrow> ('n,'t) syms \<Rightarrow> ('n,'t) syms set" where
-  "Expand_hd_syms P L \<alpha> = (case \<alpha> of [] \<Rightarrow> {[]} | x#xs \<Rightarrow> Expand_sym P L x @@ {xs})"
+  "Expand_hd_syms P X \<alpha> = (case \<alpha> of [] \<Rightarrow> {[]} | x#xs \<Rightarrow> Expand_sym P X x @@ {xs})"
 
-lemma Expand_hd_ops: "Expand_hd_syms P L \<in> Expand_ops P L"
+lemma Expand_hd_ops: "Expand_hd_syms P X \<in> Expand_ops P X"
   by (auto simp: Expand_hd_syms_def Expand_ops_def intro!: Expand_sym_ops Expand_syms_ops_self split: list.split)
 
 abbreviation Expand_hd :: "('n,'t) Prods \<Rightarrow> 'n set \<Rightarrow> ('n,'t) Prods \<Rightarrow> ('n,'t) Prods" where
-  "Expand_hd P L Q \<equiv> Expand (Expand_hd_syms P L) Q"
+  "Expand_hd P X Q \<equiv> Expand (Expand_hd_syms P X) Q"
 
 theorem Lang_Expand_hd:
-  assumes "Lhss Q \<subseteq> L"
-  shows "Lang (Expand_hd P L Q \<union> P) = Lang (Q \<union> P)"
+  assumes "X \<inter> Lhss Q = {}"
+  shows "Lang (Expand_hd P X Q \<union> P) = Lang (Q \<union> P)"
   using Lang_Expand_Un[OF Expand_hd_ops assms].
 
 end
